Fix the base of the case studies

io/case-studies/Shared.fst
@@ -5,7 +5,6 @@ open FStar.Tactics
 open Common
 open IO.Sig
 open TC.Monitorable
-open Model
 
 let rec is_open (fd:file_descr) (h: trace) : Tot bool =
   match h with
@@ -36,16 +35,11 @@ let ctx_post : file_descr -> trace -> r:(maybe unit) -> trace -> Tot (b:bool{r =
     | Inr Contract_failure -> true
     | _ -> is_open fd (apply_changes h lt)
 
-let i : model.interface = {
-  ctx_arg = file_descr;
-  ctx_ret = unit;
-  ret = unit;
-}
 
 val pi : monitorable_prop
-let pi h action =
-  match action with
-  | (| Openfile, arg |) -> 
+let pi cmd arg h =
+  match cmd with
+  | Openfile -> 
     let (fnm, _, _) : io_args Openfile = arg in not (fnm = "/etc/passwd")
   | _ -> true
 
@@ -55,38 +49,24 @@ instance ctx_post_monitorable () : monitorable_post ctx_pre (fun x h r lt -> ctx
   c2post = ();
 }
 
-let m : model.monitor i = {
-  pi = pi;
-  pre = ctx_pre;
-  post = (fun fd h r lt -> ctx_post fd h r lt);
-  post_c = ctx_post_monitorable () 
+noeq type shared_interface = {
+  ctx_arg : Type;
+  ctx_ret : Type;
+  ret : Type;
+  pi : monitorable_prop;
+  piprop : squash (forall h cmd arg. pi cmd arg h ==> io_pre cmd arg h);
+  pre : ctx_arg -> trace -> Type0;
+  post : ctx_arg -> trace -> r:(maybe ctx_ret) -> trace -> b:Type0{r == Inr Contract_failure ==> b};
+  post_c : monitorable_post pre post pi;
 }
 
-(** The following pi is too hardcore for our current state. 
-    This pi implies to have pre-/post- conditions that keep track of what
-    file descriptors are open or not. But, the plugin can close some of those
-    file descriptors and we can not prevent this bad behavior. **)
-val pi' : monitorable_prop
-let pi' h action =
-  match action with
-  | (| Openfile, _ |) -> true
-  | (| Read, arg |) -> 
-    let (fd, _) : io_args Read = arg in is_open fd h
-
-  | (| Write, arg |) -> 
-    let (fd, _) : io_args Write = arg in is_open fd h
-
-  | (| Close, fd |) -> is_open fd h
-  | (| Socket, _ |) -> true
-  | (| Setsockopt, arg |) ->
-    let (fd, _, _) : io_args Setsockopt = arg in is_open fd h
-  
-  | (| Bind, arg |) ->
-    let (fd, _, _) : io_args Bind = arg in is_open fd h
-
-  | (| SetNonblock, fd |) -> is_open fd h
-  | (| Listen, arg |) ->
-    let (fd, _) : io_args Listen = arg in is_open fd h
-  
-  | (| Accept, fd |) -> is_open fd h
-  | (| Select, _ |) -> true
+let shr : shared_interface = {
+  ctx_arg = file_descr;
+  ctx_ret = unit;
+  ret = unit;
+  pi = pi;
+  piprop = admit ();
+  pre = ctx_pre;
+  post = (fun fd h r lt -> ctx_post fd h r lt);
+  post_c = ctx_post_monitorable ()
+}
