io/case-studies/Utils.fst
@@ -1,0 +1,45 @@
+module Utils
+
+open FStar.List
+
+open DM
+open IO.Sig.Call
+
+let lemma_append_enforced_locally pi :
+  Lemma (forall h lt1 lt2.
+    enforced_locally pi h lt1 /\
+    enforced_locally pi (apply_changes h lt1) lt2 ==> 
+    enforced_locally pi h (lt1 @ lt2)) = admit () 
+
+open FStar.Tactics
+
+let static_cmd
+  (cmd : io_cmds)
+  (pi : monitorable_prop)
+  (arg : io_sig.args cmd) :
+  IO (io_resm cmd)
+    (requires (fun h -> pi cmd arg h /\ io_pre cmd arg h))
+    (ensures (fun h (r:io_sig.res cmd arg) lt ->
+        lt == [convert_call_to_event cmd arg r] /\
+        enforced_locally pi h lt)) =
+  admit ();
+  static_cmd cmd arg
+
+let io_post
+  (#a:Type)
+  (pi : monitorable_prop)
+  (h:trace)
+  (result:a)
+  (local_trace:trace) :
+  Tot bool =
+  enforced_locally pi h local_trace
+
+effect IOpi
+  (a:Type)
+  (pi : monitorable_prop)
+  (pre : trace -> Type0)
+  (post : trace -> a -> trace -> Type0) =
+  IOwp a
+    (fun p h ->
+      pre h /\
+      (forall r lt. (io_post pi h r lt /\ post h r lt) ==> p lt r))
